Remove le from Abstractdomain: we don't need it.

src/AbstractDomain.v
@@ -1,56 +1,69 @@
 From Coq Require Import ssreflect ssrfun ssrbool.
-Require Export Coq.Sets.Ensembles.
+From Coq Require Export Ensembles.
 From Coq Require Import ssrbool.
 From mathcomp Require Export eqtype.
 
 (* The abstract domain *)
 Class adom (concrete_state abstract_state: eqType) :=
   {
-    le : abstract_state -> abstract_state -> bool;
     bot : abstract_state;
     top : abstract_state;
     join : abstract_state -> abstract_state -> abstract_state;
 
     gamma : abstract_state -> Ensemble concrete_state;
 
-    le_refl: forall a, le a a;
-    le_trans: forall a1 a2 a3, le a1 a2 -> le a2 a3 -> le a1 a3;
-    gamma_monotone : forall a1 a2, le a1 a2 <-> Included concrete_state (gamma a1) (gamma a2);
     gamma_top : forall x, Ensembles.In concrete_state (gamma top) x;
     gamma_bot : forall x, ~ Ensembles.In concrete_state (gamma bot) x;
-    join_sound_l : forall a1 a2, le a1 (join a1 a2);
-    join_sound_r : forall a1 a2, le a2 (join a1 a2);
+    join_sound_l : forall a1 a2, Included _ (gamma a1) (gamma (join a1 a2));
+    join_sound_r : forall a1 a2, Included _ (gamma a2) (gamma (join a1 a2));
   }.
 
-Hint Resolve le_refl gamma_monotone gamma_top join_sound_l join_sound_r : core.
+Hint Resolve gamma_top join_sound_l join_sound_r : core.
 
 Section AbstractDomainTheorems.
 
   Context {concrete_state abstract_state: eqType}
-          (ad: adom concrete_state abstract_state).
+          {ad: adom concrete_state abstract_state}.
+
+  Definition le := (fun a1 a2 => Included _ (gamma a1) (gamma a2)).
+
+  Theorem le_refl :
+    forall a, le a a.
+  Proof.
+    move => a.
+      by rewrite /le /Included.
+  Qed.
+
+  Theorem le_trans :
+    forall a1 a2 a3, le a1 a2 -> le a2 a3 -> le a1 a3.
+  Proof.
+    move => a1 a2 a3 Hle1 Hle2 x Hin1.
+      by auto.
+  Qed.
 
   Theorem le_join_l :
     forall a1 a2 a3, le a1 a2 -> le a1 (join a2 a3).
   Proof.
-    move => a1 a2 a3 Hle.
-    by eapply le_trans; eauto.
+    move => /= a1 a2 a3 Hle.
+    eapply le_trans. apply Hle.
+    by apply join_sound_l.
   Qed.
 
   Theorem le_join_r :
     forall a1 a2 a3, le a1 a2 -> le a1 (join a3 a2).
   Proof.
     move => a1 a2 a3 Hle.
-    by eapply le_trans; eauto.
+    eapply le_trans. by apply Hle.
+    by apply join_sound_r.
   Qed.
 
   Theorem le_bot :
     forall a, le bot a.
   Proof.
-    move => a.
-    apply gamma_monotone => R HIn. exfalso.
-      by eapply gamma_bot; eauto.
+    move => a x Hin.
+      by apply gamma_bot in Hin.
   Qed.
 
 End AbstractDomainTheorems.
 
-Hint Resolve le_join_l le_join_r le_bot : core.
+Hint Resolve le_refl le_join_l le_join_r le_bot : core.
